Cleaned up BiInv.v

theories/Equiv/BiInv.v
@@ -7,132 +7,119 @@ Generalizable Variables A B f.
 
 (** A map is "bi-invertible" if it has both a section and a retraction, not necessarily the same.  This definition of equivalence was proposed by Andre Joyal. *)
 
-Definition BiInv {A B : Type} (f : A -> B) : Type
-  := {g : B -> A & g o f == idmap} * {h : B -> A & f o h == idmap}.
+Class IsBiInv {A B : Type} (f : A -> B) := {
+  sect_biinv : B -> A ;
+  retr_biinv : B -> A ;
+  eisretr_biinv : f o sect_biinv == idmap ;
+  eissect_biinv : retr_biinv o f == idmap ;
+}.
 
-Existing Class BiInv.
+Arguments sect_biinv {A B}%_type_scope f%_function_scope {_} _.
+Arguments retr_biinv {A B}%_type_scope f%_function_scope {_} _.
+Arguments eisretr {A B}%_type_scope f%_function_scope {_} _.
+Arguments eissect {A B}%_type_scope f%_function_scope {_} _.
+Arguments IsBiInv {A B}%_type_scope f%_function_scope.
 
-(** It seems that the easiest way to show that bi-invertibility is equivalent to being an equivalence is also to show that both are h-props and that they are logically equivalent. *)
+
+(** If [e] is bi-invertible, then the retraction and the section of [e] are equal. *)
+Definition sec_ret_homotopic_binv {A B : Type} (f : A -> B) `{bi : !IsBiInv f}
+  : sect_biinv f == retr_biinv f.
+Proof.
+  revert bi.
+  intros [h g r s].
+  exact (fun y => (s (h y))^ @ ap g (r y)).
+Defined.
+
+
+(** The record is equivalent to a product type. This is used below in a 'product of contractible types is contractible' argument.*)
+Definition prod_isbiinv (A B : Type) `{f: A -> B}
+  :  {g : B -> A & g o f == idmap} * {h : B -> A & f o h == idmap} <~>  IsBiInv f.
+Proof.
+    make_equiv.
+Defined.
+
+Record EquivBiInv A B := {
+  equiv_fun_biinv :> A -> B ;
+  equiv_isequiv_biinv :> IsBiInv equiv_fun_biinv
+}.
+
+Existing Instance equiv_isequiv_biinv.
+
+Definition issig_equivbiinv (A B : Type)
+  : {f : A -> B & IsBiInv f} <~> EquivBiInv A B.
+Proof.
+  issig.
+Defined.
 
 (** From a bi-invertible map, we can construct a half-adjoint equivalence in two ways. Here we take the inverse to be the retraction. *)
-Global Instance isequiv_biinv {A B : Type} (f : A -> B) `{bi : !BiInv f} : IsEquiv f.
+Global Instance isequiv_biinv {A B : Type} (f : A -> B) `{bi : !IsBiInv f} : IsEquiv f.
 Proof.
-  destruct bi as [[g s] [h r]].
+  revert bi.
+  intros [h g r s].
   exact (isequiv_adjointify f g
     (fun x => ap f (ap g (r x)^ @ s (h x)) @ r x)
     s).
 Defined.
 
+(** Here we take the inverse to be the section. *)
+Definition isequiv_biinv' {A B : Type} (f : A -> B) `{bi : !IsBiInv f} : IsEquiv f.
+Proof.
+  snrapply isequiv_adjointify.
+  - apply (sect_biinv f).
+  - apply eisretr_biinv.  (* We provide proof of eissect, but it gets modified. *)
+  - intro a.
+    lhs nrapply sec_ret_homotopic_binv.
+    apply eissect_biinv.
+Defined.
 
 Definition biinv_isequiv `(f : A -> B)
-  : IsEquiv f -> BiInv f.
+  : IsEquiv f -> IsBiInv f.
 Proof.
   intros [g s r adj].
-  exact ((g; r), (g; s)).
+  exact (Build_IsBiInv _ _ f g g s r).
 Defined.
 
 Definition iff_biinv_isequiv `(f : A -> B)
-  : BiInv f <-> IsEquiv f.
+  : IsBiInv f <-> IsEquiv f.
 Proof.
   split.
   - apply isequiv_biinv.
   - apply biinv_isequiv.
 Defined.
 
-Global Instance ishprop_biinv `{Funext} `(f : A -> B) : IsHProp (BiInv f) | 0.
+Global Instance ishprop_biinv `{Funext} `(f : A -> B) : IsHProp (IsBiInv f) | 0.
 Proof.
   apply hprop_inhabited_contr.
   intros bif.
-  apply @contr_prod.
+  srapply contr_equiv'.
+  - exact ({g : B -> A & g o f == idmap} * {h : B -> A & f o h == idmap}).
+  - exact (prod_isbiinv A B).
+  - apply @contr_prod.
   (* For this, we've done all the work already. *)
-  - rapply contr_retr_equiv.
-  - rapply contr_sect_equiv.
+    + rapply contr_retr_equiv.
+    + rapply contr_sect_equiv.
 Defined.
 
 Definition equiv_biinv_isequiv `{Funext} `(f : A -> B)
-  : BiInv f <~> IsEquiv f.
+  : IsBiInv f <~> IsEquiv f.
 Proof.
   apply equiv_iff_hprop_uncurried, iff_biinv_isequiv.
 Defined.
 
-
-(** These are some projections *)
-(* jTODO Eventually  make a Record with fields with appropriate names,
-trying to parallel Equiv and IsEquiv as much as possible.  E.g. instead of "issec_binv"
-use "eissect_biinv" with the "e" and the start and the "t" at the end.  And I think
-it should be "_biinv", not "_binv". *)
-(* TODO: The "BiInv f" parts should be moved to the left of the colon and be made implicit. "f" should be explicit. *)
-Definition ret_binv `{f : A -> B}
-  : BiInv f -> (B -> A).
-Proof.
-  intro X.
-  exact (pr1 (fst X)).
-Defined.
-
-Definition sec_binv `{f : A -> B}
-  : BiInv f -> (B -> A).
-Proof.
-  intro X.
-  exact (pr1 (snd X)).
-Defined.
-
-Definition isret_binv `{f : A -> B}
-  : forall (e: BiInv f), f o (sec_binv e) == idmap.
-Proof.
-  intro.
-  simpl.
-  exact (pr2 (snd e)).
-Defined.
-
-Definition issec_binv `{f : A -> B}
-  : forall (e: BiInv f), (ret_binv e) o f == idmap.
-Proof.
-  intro.
-  simpl.
-  exact (pr2 (fst e)).
-Defined.
-
-
-(** A record summing over all bi-invertible maps*)
-
-Record EquivBiInv A B := {
-  equiv_fun_binv :> A -> B ;
-  equiv_isequiv_binv :> BiInv equiv_fun_binv
-}.
-
-Existing Instance equiv_isequiv_binv.
-
-Definition issig_equivbiinv (A B : Type)
-  : {f : A -> B & BiInv f} <~> EquivBiInv A B.
-Proof.
-  issig.
-Defined.
-
 (* Some lemmas to send equivalences and biinvertible maps back and forth.*)
 
-(* TODO: This should be called equiv_ not isequiv_ *)
-Definition isequiv_biinv_record A B (f : EquivBiInv A B)
+Definition equiv_biinv A B (f : EquivBiInv A B)
   : A <~> B
   := Build_Equiv A B f _.
 
-(* TODO: change isequiv to equiv in name: *)
-Definition biinv_isequiv_record A B
+Definition biinv_equiv A B
   :  A <~> B -> EquivBiInv A B.
 Proof.
   intros [f e].
   exact (Build_EquivBiInv A B f (biinv_isequiv f e)).
 Defined.
 
-(* TODO: Delete this.  "iff" is useful between hprops, but not in cases like this. *)
-Definition iff_biinv_isequiv_record A B
-  : EquivBiInv A B <-> A <~> B.
-Proof.
-  split.
-  - apply isequiv_biinv_record.
-  - apply biinv_isequiv_record.
-Defined.
-
-Definition equiv_biinv_isequiv_record `{Funext} A B
+Definition equiv_biinv_equiv `{Funext} A B
   : EquivBiInv A B <~> (A <~> B) .
 Proof.
   refine ((issig_equiv A B) oE _ oE (issig_equivbiinv A B)^-1).
@@ -142,50 +129,8 @@ Defined.
 Definition equiv_idmap_binv (A : Type) 
   : (EquivBiInv A A).
 Proof.
-  by nrefine (Build_EquivBiInv A A idmap ((idmap; _), (idmap; _))).
+  by nrefine (Build_EquivBiInv A A idmap (Build_IsBiInv A A idmap idmap idmap _ _ )).
 Defined.
-
-
-(** TODO chnage BiInv to IsBinv and make it also a record*)
-(** A typeclass that includes the data making [f] into a bi-invertible equivalence.
-Class IsBinv {A B : Type} (f : A -> B) := {
-  sec_proj : B -> A ;
-  ret_proj : B -> A ;
-  eisretr : f o sec_proj == idmap ;
-  eissect : ret_proj o f == idmap ;
-}.
-
-Record EquivBiInv A B := {
-  equiv_fun_binv : A -> B ;
-  equiv_isequiv_binv : IsBinv equiv_fun_binv
-}. *)
-
-
-Section BiInvProperties.
-
-  (* TODO: The following things should go right after the definition of BiInv, but they are here so I can make use of the accessor functions.  They are no longer needed in the proof below, but should probably still be part of the general theory of bi-invertible maps.  In particular, it seems like it might be useful to have isequiv_biinv'. *)
-
-  (** If [e] is bi-invertible, then the retraction and the section of [e] are equal. *)
-  Definition sec_ret_homotopic_binv {A B : Type} (f : A -> B) `{bi : !BiInv f}
-    : sec_binv bi == ret_binv bi.
-  Proof.
-    destruct bi as [[g s] [h r]].
-    exact (fun y => (s (h y))^ @ ap g (r y)).
-  Defined.
-
-(** TODO move up after definition*)
-(** Here we take the inverse to be the section. *)
-Definition isequiv_biinv' {A B : Type} (f : A -> B) `{bi : !BiInv f} : IsEquiv f.
-Proof.
-  snrapply isequiv_adjointify.
-  - apply (sec_binv bi).
-  - apply isret_binv.  (* We provide proof of eissect, but it gets modified. *)
-  - intro a.
-    lhs nrapply sec_ret_homotopic_binv.
-    apply issec_binv.
-Defined.
-
-End BiInvProperties.
 
 (* TODO: move this to right after equiv_inj in PathGroupoids.v *)
 Definition equiv_inj_comp `(f : A -> B) `{IsEquiv A B f} {x y : A}
@@ -196,19 +141,19 @@ Proof.
   apply eisretr.
 Defined.
 
-Section DansAttempt.
+Section EquivalenceCompatibility.
 
   Context (A B C D : Type).
   Context (e : EquivBiInv A B) (e' : EquivBiInv C D) (f : A -> C) (g : B -> D).
 
-  Let s := sec_binv e.
-  Let r := ret_binv e.
-  Let re := issec_binv e : r o e == idmap.
-  Let es := isret_binv e : e o s == idmap.
-  Let s' := sec_binv e'.
-  Let r' := ret_binv e'.
-  Let re' := issec_binv e' : r' o e' == idmap.
-  Let es' := isret_binv e' : e' o s' == idmap.
+  Let s := sect_biinv e.
+  Let r := retr_biinv e.
+  Let re := eissect_biinv : r o e == idmap.
+  Let es := eisretr_biinv : e o s == idmap.
+  Let s' := sect_biinv e'.
+  Let r' := retr_biinv e'.
+  Let re' := eissect_biinv : r' o e' == idmap.
+  Let es' := eisretr_biinv : e' o s' == idmap.
 
   Definition helper_r (pe : e' o f == g o e) : r' o g o e == f o r o e.
   Proof.
@@ -231,7 +176,7 @@ Section DansAttempt.
     pes : forall (y : B), es' (g y) = ap e' (ps y) @ pe (s y) @ ap g (es y);
   }.
 
-  Definition compat_implies_prBiInv' (pe : forall (x : A), e' (f x) = g (e x))
+  Definition compat_implies_prBiInv (pe : forall (x : A), e' (f x) = g (e x))
     : prBiInv.
   Proof.
     srapply Build_prBiInv.
@@ -253,96 +198,60 @@ Section DansAttempt.
       reflexivity.
   Defined.
 
-End DansAttempt.
+End EquivalenceCompatibility.
 
 
-Section BiInvCompatUnivalence.
-Context `{Univalence}.
+(** ---------------------------------------------------------------------------------------- *)
+(** The following is the old type that is used elsewhere in the library. It is left here so everything compiles*)
 
-(* Definition equiv_path_binv (A B : Type@{u}) (p : A = B) : EquivBiInv A B 
-  := (((equiv_fun (equiv_biinv_isequiv_record A B)^-1) o (equiv_path A B)) p). *)
+(** * Bi-invertible maps *)
 
-Definition equiv_path_binv (A B : Type@{u}) : (A = B) <~> EquivBiInv A B
-  := (equiv_biinv_isequiv_record A B)^-1 oE equiv_equiv_path A B. 
+(** A map is "bi-invertible" if it has both a section and a retraction, not necessarily the same.  This definition of equivalence was proposed by Andre Joyal. *)
 
+Definition BiInv {A B : Type} (f : A -> B) : Type
+  := {g : B -> A & g o f == idmap} * {h : B -> A & f o h == idmap}.
 
-(** Paulin-Mohring style *)
-Theorem equiv_induction_binv {U : Type} (P : forall V, EquivBiInv U V -> Type)
-  : (P U (equiv_idmap_binv U)) -> (forall V (w :  EquivBiInv U V), P V w).
+Existing Class BiInv.
+
+(** It seems that the easiest way to show that bi-invertibility is equivalent to being an equivalence is also to show that both are h-props and that they are logically equivalent. *)
+
+(** From a bi-invertible map, we can construct a half-adjoint equivalence in two ways. Here we take the inverse to be the retraction. *)
+Global Instance isequiv_biinv'' {A B : Type} (f : A -> B) `{bi : !BiInv f} : IsEquiv f.
 Proof.
-  intros H0 V w.
-  srapply (equiv_ind (equiv_path_binv U V)).
-  - intro p.
-    induction p.
-    exact H0.
-Defined.
-
-(** Martin-Lof style *)
-Theorem equiv_induction_binv' 
-  (P : forall U V, (EquivBiInv U V) -> Type)
-  : (forall T, P T T (equiv_idmap_binv T)) -> (forall U V (w : (EquivBiInv U V)), P U V w).
-Proof.
-  intros H0 U V w.
-  srapply (equiv_ind (equiv_path_binv U V)).
-  - intro p.
-    induction p.
-    apply H0.
+  destruct bi as [[g s] [h r]].
+  exact (isequiv_adjointify f g
+    (fun x => ap f (ap g (r x)^ @ s (h x)) @ r x)
+    s).
 Defined.
 
 
-(** Bi-Invertible maps*)
-Definition compat_implies_prBiInv
-  (A B C D: Type)
-  (e: EquivBiInv A B)
-  (e':  EquivBiInv C D)
-  (a: A -> C)
-  (b : B -> D)
-  :
-    (forall (x : A), (e' o a) x = (b o e) x) -> prBiInv A B C D e e' a b.
+Definition biinv_isequiv' `(f : A -> B)
+  : IsEquiv f -> BiInv f.
 Proof.
-  revert b.  
-  generalize dependent e.
-  revert B.
-  snrapply equiv_induction_binv.
-  generalize dependent e'.
-  revert D.
-  snrapply equiv_induction_binv.
-  simpl.
-  intros b K.
-  snrapply Build_prBiInv.
-  - simpl.
-    exact K.
-  - intro y.
-    simpl.
-    exact (K y)^.
-  - intro y.
-    simpl. 
-    exact (K y)^.
-  - simpl.
-    intro x.
-    rewrite ap_idmap.
-    rewrite concat_pV.
-    reflexivity.
-  - simpl. (* induction (H y). causes a bug here *)
-    intro y.
-    rewrite ap_idmap.
-    rewrite concat_Vp.
-    reflexivity.
+  intros [g s r adj].
+  exact ((g; r), (g; s)).
 Defined.
 
-Definition compat_iff_prBiInv
-  (A B C D: Type)
-  (e: EquivBiInv A B)
-  (e':  EquivBiInv C D)
-  (a: A -> C)
-  (b : B -> D)
-  :
-    (forall (x : A), (e' o a) x = (b o e) x) <-> prBiInv A B C D e e' a b.
+Definition iff_biinv_isequiv' `(f : A -> B)
+  : BiInv f <-> IsEquiv f.
 Proof.
   split.
-    - exact (compat_implies_prBiInv _ _ _ _ _ _ _ _).
-    - intro K.
-      exact (pe _ _ _ _ _ _ _ _ K).
+  - apply isequiv_biinv''.
+  - apply biinv_isequiv'.
 Defined.
 
+Global Instance ishprop_biinv' `{Funext} `(f : A -> B) : IsHProp (BiInv f) | 0.
+Proof.
+  apply hprop_inhabited_contr.
+  intros bif.
+  apply @contr_prod.
+  (* For this, we've done all the work already. *)
+  - rapply contr_retr_equiv.
+  - rapply contr_sect_equiv.
+Defined.
 
+Definition equiv_biinv_isequiv' `{Funext} `(f : A -> B)
+  : BiInv f <~> IsEquiv f.
+Proof.
+  apply equiv_iff_hprop_uncurried, iff_biinv_isequiv'.
+Defined.
